Attempt2/Compose.dfy
@@ -1,7 +1,6 @@
 module Compose {
 
   import opened Circ
-  //import opened Eval
   import opened Utils
   import opened MapFunction
   import opened Equiv
@@ -18,11 +17,18 @@ module Compose {
     (NPBetweenSubcircuits(c, e1.sc, e2.sc) == {})
   }
 
-  lemma SetsNoIntersectionFromComposedValid(c: Circuit, e1: Equiv, e2: Equiv)
+  lemma {:vcs_split_on_every_assert} SetsNoIntersectionFromComposedValid(c: Circuit, e1: Equiv, e2: Equiv)
   requires ComposedValid(c, e1, e2)
   ensures SetsNoIntersection(e1.sc, e2.sc)
+  ensures SetsNoIntersection(e1.inputs, e2.inputs)
+  ensures SetsNoIntersection(e1.outputs, e2.outputs)
+  ensures SetsNoIntersection(e1.inputs, e2.outputs)
+  ensures SetsNoIntersection(e1.outputs, e2.inputs)
   {
     reveal ComposedValid();
+    reveal ScValid();
+    reveal EquivValid();
+    reveal NPsValidAndInSc();
   }
 
   lemma CircuitValidFromComposedValid(c: Circuit, e1: Equiv, e2: Equiv)
@@ -33,7 +39,7 @@ module Compose {
   }
 
 
-  function {:vcs_split_on_every_assert} ComposeEquiv(c: Circuit, e1: Equiv, e2: Equiv): (r: Equiv)
+  function ComposeEquiv(c: Circuit, e1: Equiv, e2: Equiv): (r: Equiv)
     requires ComposedValid(c, e1, e2)
     ensures EquivValid(c, r)
   {
@@ -46,6 +52,18 @@ module Compose {
       e1.outputs + e2.outputs,
       (combined_inputs: map<NP, bool>) requires combined_inputs.Keys == combined_input_keys => ComposeEquivF(c, e1, e2, combined_inputs)
     );
+    assert ScValid(c, e.sc) by {reveal ScValid();}
+    assert (ScInputBoundary(c, e.sc) == e.inputs) by {
+      ComposeEquivInputsCorrect(c, e1, e2);
+    }
+    assert SetsNoIntersection(e.inputs, e.outputs) by {
+      SetsNoIntersectionFromComposedValid(c, e1, e2);
+    }
+    assert NPsValidAndInSc(c, e.sc, e.outputs) by {reveal NPsValidAndInSc();}
+    assert NPsValidAndInSc(c, e.sc, e.inputs) by {reveal NPsValidAndInSc();}
+    assert MapFunctionValid(EtoMf(e)) by {reveal MapFunctionValid();}
+    assert EquivScOutputsInOutputs(c, e.sc, e.outputs) by {reveal EquivScOutputsInOutputs();}
+    assert EquivValid(c, e);
     e
   }
 
@@ -55,7 +73,28 @@ module Compose {
   {
     reveal ComposedValid();
     reveal EquivValid();
-    (set np | np in (e1.inputs + e2.inputs) && np !in NPBetweenSubcircuits(c, e2.sc, e1.sc))
+    (e1.inputs + e2.inputs) - NPBetweenSubcircuits(c, e2.sc, e1.sc)
+  }
+
+  lemma {:vcs_split_on_every_assert} ComposeEquivInputsCorrectHelper(c: Circuit, e1: Equiv, e2: Equiv)
+    requires ComposedValid(c, e1, e2)
+    ensures
+      ScValid(c, e1.sc) &&
+      ScValid(c, e2.sc) &&
+      ScValid(c, e1.sc + e2.sc) &&
+      NPBetweenSubcircuitsComplement(c, e1.sc + e2.sc, e1.sc + e2.sc) ==
+        NPBetweenSubcircuitsComplement(c, e1.sc, e1.sc) +
+        NPBetweenSubcircuitsComplement(c, e2.sc, e2.sc) -
+        NPBetweenSubcircuits(c, e2.sc, e1.sc)
+  {
+    reveal ComposedValid();
+    assert ScValid(c, e1.sc);
+    assert ScValid(c, e2.sc);
+    assert ScValid(c, e1.sc + e2.sc) by {reveal ScValid();}
+    assert NPBetweenSubcircuitsComplement(c, e1.sc + e2.sc, e1.sc + e2.sc) ==
+        NPBetweenSubcircuitsComplement(c, e1.sc, e1.sc) + NPBetweenSubcircuitsComplement(c, e2.sc, e2.sc) -
+        NPBetweenSubcircuits(c, e2.sc, e1.sc) - NPBetweenSubcircuits(c, e1.sc, e2.sc);
+    assert NPBetweenSubcircuits(c, e1.sc, e2.sc) == {};
   }
 
   lemma ComposeEquivInputsCorrect(c: Circuit, e1: Equiv, e2: Equiv)
@@ -65,22 +104,136 @@ module Compose {
       ScInputBoundary(c, e1.sc + e2.sc) == ComposeEquivInputs(c, e1, e2)
   {
     reveal ComposedValid();
+    assert ScValid(c, e1.sc + e2.sc) && ScValid(c, e1.sc) && ScValid(c, e2.sc) by {
+      reveal ScValid();
+    }
+    var ui := UnconnectedINPs(c, e1.sc + e2.sc) + InternalInputs(c, e1.sc + e2.sc);
+    var nb :=  NPBetweenSubcircuitsComplement(c, e1.sc, e1.sc) +
+               NPBetweenSubcircuitsComplement(c, e2.sc, e2.sc) -
+               NPBetweenSubcircuits(c, e2.sc, e1.sc);
+    calc {
+      ComposeEquivInputs(c, e1, e2);
+      (e1.inputs + e2.inputs) - NPBetweenSubcircuits(c, e2.sc, e1.sc);
+      {reveal EquivValid();}
+      ScInputBoundary(c, e1.sc) + ScInputBoundary(c, e2.sc)
+        - NPBetweenSubcircuits(c, e2.sc, e1.sc);
+      NPBetweenSubcircuitsComplement(c, e1.sc, e1.sc) +
+        UnconnectedINPs(c, e1.sc) + InternalInputs(c, e1.sc) +
+        NPBetweenSubcircuitsComplement(c, e2.sc, e2.sc) +
+        UnconnectedINPs(c, e2.sc) + InternalInputs(c, e2.sc) -
+        NPBetweenSubcircuits(c, e2.sc, e1.sc);
+      UnconnectedINPs(c, e1.sc + e2.sc) + InternalInputs(c, e1.sc + e2.sc) +
+        NPBetweenSubcircuitsComplement(c, e1.sc, e1.sc) +
+        NPBetweenSubcircuitsComplement(c, e2.sc, e2.sc) -
+        NPBetweenSubcircuits(c, e2.sc, e1.sc);
+      {
+        // Need to show that the terms in NPBetweenSubcircuits are not in Unconnected or Internal.
+        assert forall np :: np in UnconnectedINPs(c, e1.sc + e2.sc) ==> np !in c.PortSource;
+        reveal CircuitValid();
+        assert forall np :: np in InternalInputs(c, e1.sc + e2.sc) ==> np !in c.PortSource;
+        assert forall np :: np in NPBetweenSubcircuits(c, e2.sc, e1.sc) ==> np in c.PortSource;
+      }
+      UnconnectedINPs(c, e1.sc + e2.sc) + InternalInputs(c, e1.sc + e2.sc) +
+        (NPBetweenSubcircuitsComplement(c, e1.sc, e1.sc) +
+        NPBetweenSubcircuitsComplement(c, e2.sc, e2.sc) -
+        NPBetweenSubcircuits(c, e2.sc, e1.sc));
+      {ComposeEquivInputsCorrectHelper(c, e1, e2);}
+      UnconnectedINPs(c, e1.sc + e2.sc) + InternalInputs(c, e1.sc + e2.sc) +
+        NPBetweenSubcircuitsComplement(c, e1.sc + e2.sc, e1.sc + e2.sc);
+      ScInputBoundary(c, e1.sc + e2.sc);
+    }
+  }
+
+  lemma ONPNotInKnownsNotInKnowns2(c: Circuit, onp: NP, e1: Equiv, e2: Equiv, knowns: map<NP, bool>)
+    requires ComposedValid(c, e1, e2)
+    requires GoodKnownKeys(c, e1, e2, knowns)
+    requires onp !in knowns
+    requires ONPValid(c, onp)
+    ensures onp !in CalculateE2Inputs(c, e1, e2, knowns)
+  {
+    reveal ComposedValid();
+    reveal GoodKnownKeys();
+    assert (onp !in (e1.inputs + e2.inputs) - NPBetweenSubcircuits(c, e2.sc, e1.sc));
+    var knowns_2 := CalculateE2Inputs(c, e1, e2, knowns);
+    var e2_inputs_from_e1_keys := NPBetweenSubcircuits(c, e2.sc, e1.sc);
+    assert forall np :: np in knowns_2 ==> np in e2_inputs_from_e1_keys || np in knowns;
+    assert onp !in e2_inputs_from_e1_keys by {
+      reveal CircuitValid();
+    }
+  }
+
+  opaque predicate GoodKnownKeys(c: Circuit, e1: Equiv, e2: Equiv, knowns: map<NP, bool>)
+    requires ComposedValid(c, e1, e2)
+  {
+    knowns.Keys == ComposeEquivInputs(c, e1, e2)
+  }
+
+  lemma InE1ButNotE1InputsNotInKnowns(c: Circuit, e1: Equiv, e2: Equiv, knowns: map<NP, bool>, np: NP)
+    requires ComposedValid(c, e1, e2)
+    requires GoodKnownKeys(c, e1, e2, knowns)
+    requires np.n in e1.sc
+    requires np !in e1.inputs
+    ensures np !in knowns
+  {
+    reveal ComposedValid();
+    reveal GoodKnownKeys();
+    reveal ScValid();
+    InThisNotInThat(np.n, e1.sc, e2.sc);
+    assert np.n !in e2.sc;
+    assert knowns.Keys == (e1.inputs + e2.inputs) - NPBetweenSubcircuits(c, e2.sc, e1.sc);
     reveal EquivValid();
+    reveal NPsValidAndInSc();
+    assert np !in e2.inputs;
+  }
+
+  lemma InE2ButNotE2InputsNotInKnowns(c: Circuit, e1: Equiv, e2: Equiv, knowns: map<NP, bool>, np: NP)
+    requires ComposedValid(c, e1, e2)
+    requires GoodKnownKeys(c, e1, e2, knowns)
+    requires np.n in e2.sc
+    requires np !in e2.inputs
+    ensures np !in knowns
+  {
+    reveal ComposedValid();
+    reveal GoodKnownKeys();
+    reveal ScValid();
+    InThisNotInThat(np.n, e2.sc, e1.sc);
+    assert np.n !in e1.sc;
+    assert knowns.Keys == (e1.inputs + e2.inputs) - NPBetweenSubcircuits(c, e2.sc, e1.sc);
+    reveal EquivValid();
+    reveal NPsValidAndInSc();
+    assert np !in e2.inputs;
   }
 
   function CalculateE2Inputs(c: Circuit, e1: Equiv, e2: Equiv, knowns: map<NP, bool>): (r: map<NP, bool>)
     requires ComposedValid(c, e1, e2)
-    requires knowns.Keys == ComposeEquivInputs(c, e1, e2)
+    requires GoodKnownKeys(c, e1, e2, knowns)
   {
     reveal ComposedValid();
     reveal EquivValid();
-    var mf1 := MapFunction(e1.inputs, e1.outputs, e1.f);
-    var mf2 := MapFunction(e2.inputs, e2.outputs, e2.f);
+    reveal CircuitValid();
+    reveal GoodKnownKeys();
+    var mf1 := EtoMf(e1);
+    var mf2 := EtoMf(e2);
     assert MapFunctionValid(mf1);
     assert MapFunctionValid(mf2);
     var e2_inputs_from_e1_keys := NPBetweenSubcircuits(c, e2.sc, e1.sc);
     var e2_inputs_from_e1 := (map np | np in e2_inputs_from_e1_keys :: np := c.PortSource[np]);
+    assert forall np :: np in e2_inputs_from_e1_keys ==> np in e2.inputs;
+    assert forall np :: np in e2_inputs_from_e1.Values ==> np in e1.outputs by {
+      reveal EquivScOutputsInOutputs();
+    }
+    assert SetsNoIntersection(mf1.inputs+mf1.outputs, mf2.inputs+mf2.outputs) by {
+      reveal NPsValidAndInSc();
+    }
     GetInputs2(mf1, mf2, e2_inputs_from_e1, knowns)
+  }
+
+  lemma CalculateE2InputsKeysCorrect(c: Circuit, e1: Equiv, e2: Equiv, knowns: map<NP, bool>)
+    requires ComposedValid(c, e1, e2)
+    requires GoodKnownKeys(c, e1, e2, knowns)
+    ensures
+      CalculateE2Inputs(c, e1, e2, knowns).Keys == e2.inputs
+  {
   }
 
   function ComposeEquivF(c: Circuit, e1: Equiv, e2: Equiv, combined_inputs: map<NP, bool>): (r: map<NP, bool>)
@@ -95,6 +248,16 @@ module Compose {
     assert MapFunctionValid(mf2);
     var e2_inputs_from_e1_keys := NPBetweenSubcircuits(c, e2.sc, e1.sc);
     var e2_inputs_from_e1 := (map np | np in e2_inputs_from_e1_keys :: np := c.PortSource[np]);
+    assert forall np :: np in e2_inputs_from_e1_keys ==> np in e2.inputs by {
+      reveal CircuitValid();
+    }
+    assert forall np :: np in e2_inputs_from_e1.Values ==> np in e1.outputs by {
+      reveal EquivScOutputsInOutputs();
+      reveal CircuitValid();
+    }
+    assert SetsNoIntersection(mf1.inputs+mf1.outputs, mf2.inputs+mf2.outputs) by {
+      reveal NPsValidAndInSc();
+    }
     ComposeMapFunction(mf1, mf2, e2_inputs_from_e1, combined_inputs)
   }
 }
