Attempt2/Connecting.dfy
@@ -2,6 +2,10 @@ module Connecting {
 
   import opened Circ
   import opened ConservedSubcircuit
+  import opened Utils
+  import opened Equiv
+  import opened Compose
+  import opened ComposeEval
 
   lemma ConnectPreservesSubcircuit(c: Circuit, inp: NP, onp: NP, sc: set<CNode>)
     requires CircuitValid(c)
@@ -14,15 +18,89 @@ module Connecting {
       var r := Connect(c, inp, onp);
       SubcircuitConserved(c, r, sc)
   {
-    var ca := c;
-    var cb := Connect(c, inp, onp);
-    assert (forall n :: n in sc ==> n in ca.NodeKind && n in cb.NodeKind);
-    assert (forall n :: n in sc ==> ca.NodeKind[n] == cb.NodeKind[n]);
-    assert (forall n :: n in sc ==> ca.NodeKind[n] == cb.NodeKind[n]);
-    assert (forall np: NP :: (np in ScInputBoundary(ca, sc)) == (np in ScInputBoundary(cb, sc)));
-    assert (forall np: NP :: (np !in ScInputBoundary(ca, sc)) && np.n in sc ==> (np in ca.PortSource) == (np in cb.PortSource));
-    assert (forall np: NP :: (np !in ScInputBoundary(ca, sc)) && np.n in sc && np in ca.PortSource ==> ca.PortSource[np] == cb.PortSource[np]);
+    reveal CircuitValid();
+    reveal ScValid();
+    reveal SubcircuitConserved();
   }
 
+  function ConnectMany(c: Circuit, connection: map<NP, NP>): (r: Circuit)
+    requires CircuitValid(c)
+    requires forall np :: np in connection.Keys ==> np !in c.PortSource
+    requires forall np :: np in connection.Keys ==> INPValid(c, np)
+    requires forall np :: np in connection.Values ==> ONPValid(c, np)
+    ensures CircuitValid(r)
+  {
+    reveal CircuitValid();
+    var new_c := Circuit(
+      c.NodeKind,
+      AddMaps(c.PortSource, connection)
+    );
+    assert (forall np :: np in new_c.PortSource.Values ==> ONPValid(c, np));
+    assert (forall np :: np in new_c.PortSource.Keys ==> INPValid(c, np));
+    new_c
+  }
+
+  lemma ConnectManyScOutputBoundary(c: Circuit, connection: map<NP, NP>, sc: set<CNode>)
+    requires CircuitValid(c)
+    requires forall np :: np in connection.Keys ==> np !in c.PortSource
+    requires forall np :: np in connection.Keys ==> INPValid(c, np)
+    requires forall np :: np in connection.Values ==> ONPValid(c, np)
+    // No connections from the sc
+    requires forall np :: np in connection.Keys ==> np.n !in sc
+    ensures
+      var new_c := ConnectMany(c, connection);
+      var new_outputs := (set np | np in connection.Values && np.n in sc :: np);
+
+      ScOutputBoundary(c, sc) + new_outputs == ScOutputBoundary(new_c, sc)
+  {
+  }
+
+  lemma ConnectManyConservesSubcircuit(c: Circuit, connection: map<NP, NP>, sc: set<CNode>)
+    requires CircuitValid(c)
+    requires ScValid(c, sc)
+    requires forall np :: np in connection.Keys ==> np !in c.PortSource
+    requires forall np :: np in connection.Keys ==> INPValid(c, np)
+    requires forall np :: np in connection.Values ==> ONPValid(c, np)
+    // It shouldn't effect an equiv as long as it doesnt create an internal connection in the equiv or
+    requires forall np :: (np in connection.Keys && np.n in sc) ==> connection[np].n !in sc
+    ensures SubcircuitConserved(c, ConnectMany(c, connection), sc)
+  {
+    reveal CircuitValid();
+    reveal SubcircuitConserved();
+    reveal ScValid();
+  }
+
+  function ConnectEquivs(c: Circuit, e1: Equiv, e2: Equiv, connection: map<NP, NP>): (r: (Circuit, Equiv))
+    requires CircuitValid(c)
+    requires EquivValid(c, e1) && EquivTrue(c, e1)
+    requires EquivValid(c, e2) && EquivTrue(c, e2)
+    requires SetsNoIntersection(e1.sc, e2.sc)
+    requires ScValid(c, e1.sc)
+    requires ScValid(c, e2.sc)
+    requires (NPBetweenSubcircuits(c, e1.sc, e2.sc) == {})
+    requires forall np :: np in connection.Keys ==> np !in c.PortSource
+    requires forall np :: np in connection.Keys ==> (np in e2.inputs) && INPValid(c, np)
+    requires forall np :: np in connection.Values ==> np in e1.outputs && ONPValid(c, np)
+    //requires forall np :: np in outputs_to_remove ==> np in (e1.outputs + e2.outputs)
+    ensures CircuitValid(r.0)
+    ensures EquivValid(r.0, r.1) && EquivTrue(r.0, r.1)
+    ensures SubcircuitConserved(c, r.0, SubcircuitComplement(c, e1.sc+e2.sc))
+    ensures SubcircuitUnconnected(c, r.0, SubcircuitComplement(c, e1.sc+e2.sc))
+  {
+    var new_c := ConnectMany(c, connection);
+    reveal CircuitValid();
+    reveal EquivValid();
+    reveal ScValid();
+    reveal NPsValidAndInSc();
+    reveal EquivScOutputsInOutputs();
+    ConnectManyConservesSubcircuit(c, connection, e1.sc);
+    ConnectManyConservesSubcircuit(c, connection, e2.sc);
+    EquivConserved(c, new_c, e1);
+    EquivConserved(c, new_c, e2);
+    reveal ComposedValid();
+    var intermed_e := ComposeEquiv(new_c, e1, e2);
+    ComposeEquivCorrect(new_c, e1, e2);
+    (new_c, intermed_e)
+  }
 
 }
