Attempt2/ConservedSubcircuit.dfy
@@ -3,6 +3,8 @@ module ConservedSubcircuit {
   import opened Circ
   import opened Eval
   import opened Equiv
+  import opened Utils
+  import opened MapFunction
 
   // To show that the rest of the graph is unchanged I need to show that
   // there is a set of nodes which have the same n.
@@ -16,25 +18,103 @@ module ConservedSubcircuit {
     boundary: set<NP>
   )
 
-  predicate SubcircuitValid(c: Circuit, sc: Subcircuit)
+  // What kind of changes would I like to categorize
+  // 1) This subcircuit has it's internal stucture left alone.
+  // 2) This subcircuit has no new connections in.
+  // 3) This subcircuit has no new connections out.
+  // 4) This subcircuit is totally left alone (i.e. not change or connections in or out) (1 + 2 + 3)
+
+
+  ghost opaque predicate CircuitConserved(ca: Circuit, cb: Circuit)
   {
-    (forall np :: np in sc.boundary ==> INPValid(c, np) || ONPValid(c, np)) &&
-    (forall n :: n in sc.nodes ==> n in c.NodeKind) &&
-    (forall np :: np in sc.boundary ==> np.n in sc.nodes) &&
-    (forall np: NP :: np.n in sc.nodes && np in c.PortSource && np !in sc.boundary ==>
-      c.PortSource[np].n in sc.nodes)
+    && (forall n :: n in ca.NodeKind ==> n in cb.NodeKind)
+    && (forall n :: n in ca.NodeKind ==> ca.NodeKind[n] == cb.NodeKind[n])
+    && (forall np: NP :: np in ca.PortSource ==> np in cb.PortSource && ca.PortSource[np] == cb.PortSource[np])
+    && (forall np: NP :: np.n in ca.NodeKind && np !in ca.PortSource && np in cb.PortSource ==> cb.PortSource[np].n !in ca.NodeKind)
   }
 
-  ghost predicate SubcircuitConserved(ca: Circuit, cb: Circuit, sc: set<CNode>)
+  ghost opaque predicate CircuitUnconnected(ca: Circuit, cb: Circuit)
   {
-    (forall n :: n in sc ==> n in ca.NodeKind && n in cb.NodeKind) &&
-    (forall n :: n in sc ==> ca.NodeKind[n] == cb.NodeKind[n]) &&
-    (forall np: NP :: (np in ScInputBoundary(ca, sc)) == (np in ScInputBoundary(cb, sc))) &&
-    (forall np: NP :: (np !in ScInputBoundary(ca, sc)) && np.n in sc ==> (np in ca.PortSource) == (np in cb.PortSource)) &&
-    (forall np: NP :: (np !in ScInputBoundary(ca, sc)) && np.n in sc && np in ca.PortSource ==> ca.PortSource[np] == cb.PortSource[np])
+    && (forall np :: np in cb.PortSource && np !in ca.PortSource ==> np.n !in ca.NodeKind && cb.PortSource[np].n !in ca.NodeKind)
   }
 
-  ghost predicate ConservedValid(ca: Circuit, cb: Circuit, e: Equiv, known: map<NP, bool>)
+  lemma CircuitConservedToSubcircuitConserved(ca: Circuit, cb: Circuit, sc: set<CNode>)
+    requires CircuitValid(ca)
+    requires CircuitValid(cb)
+    requires CircuitConserved(ca, cb)
+    requires ScValid(ca, sc)
+    ensures SubcircuitConserved(ca, cb, sc)
+  {
+    reveal CircuitValid();
+    reveal CircuitConserved();
+    reveal SubcircuitConserved();
+    reveal ScValid();
+  }
+
+  lemma CircuitConservedTransitive(ca: Circuit, cb: Circuit, cc: Circuit)
+    requires CircuitConserved(ca, cb)
+    requires CircuitConserved(cb, cc)
+    ensures CircuitConserved(ca, cc)
+  {
+    reveal CircuitConserved();
+  }
+
+  ghost opaque predicate SubcircuitConserved(ca: Circuit, cb: Circuit, sc: set<CNode>)
+  {
+    reveal ScValid();
+    && (forall n :: n in sc ==> n in ca.NodeKind && n in cb.NodeKind)
+    && (forall n :: n in sc ==> ca.NodeKind[n] == cb.NodeKind[n])
+    && (forall np: NP :: (np in ScInputBoundary(ca, sc)) == (np in ScInputBoundary(cb, sc)))
+    && (forall np: NP :: (np !in ScInputBoundary(ca, sc)) && np.n in sc ==> (np in ca.PortSource) == (np in cb.PortSource))
+    && (forall np: NP :: (np !in ScInputBoundary(ca, sc)) && np.n in sc && np in ca.PortSource ==> ca.PortSource[np] == cb.PortSource[np])
+  }
+
+  ghost opaque predicate SubcircuitUnconnected(ca: Circuit, cb: Circuit, sc: set<CNode>)
+  {
+    && (forall np :: np in cb.PortSource && np !in ca.PortSource ==> np.n !in sc && cb.PortSource[np].n !in sc)
+  }
+
+  ghost opaque predicate SubcircuitIsIsland(c: Circuit, sc: set<CNode>)
+  {
+    && (forall np :: np in c.PortSource && np.n in sc ==> c.PortSource[np].n in sc)
+    && (forall np :: np in c.PortSource && np.n !in sc ==> c.PortSource[np].n !in sc)
+  }
+  
+  lemma CircuitConservedSubcircuitConserved(ca: Circuit, cb: Circuit)
+    requires CircuitValid(ca)
+    requires CircuitValid(cb)
+    requires CircuitConserved(ca, cb)
+    ensures SubcircuitConserved(ca, cb, ca.NodeKind.Keys)
+  {
+    reveal CircuitValid();
+    reveal CircuitConserved();
+    reveal SubcircuitConserved();
+    reveal ScValid();
+    var sc := ca.NodeKind.Keys;
+    var nps := AllNPFromNodes(ca, sc);
+    assert nps == AllNPFromNodes(cb, sc);
+
+    // There may be some things in cb that are no longer unconnected.
+    var newly_connected := (set np | np in nps && np in cb.PortSource && np !in ca.PortSource :: np);
+
+    calc {
+      ScInputBoundary(ca, sc);
+      NPBetweenSubcircuitsComplement(ca, sc, sc) + UnconnectedINPs(ca, sc) + InternalInputs(ca, sc);
+      (NPBetweenSubcircuitsComplement(cb, sc, sc) - newly_connected) + UnconnectedINPs(ca, sc) + InternalInputs(ca, sc);
+      (NPBetweenSubcircuitsComplement(cb, sc, sc) - newly_connected) + (UnconnectedINPs(cb, sc) + newly_connected) + InternalInputs(ca, sc);
+      {assert forall np :: np in newly_connected ==> np in NPBetweenSubcircuitsComplement(cb, sc, sc) && np !in UnconnectedINPs(cb, sc);}
+      NPBetweenSubcircuitsComplement(cb, sc, sc) + UnconnectedINPs(cb, sc) + InternalInputs(ca, sc);
+      NPBetweenSubcircuitsComplement(cb, sc, sc) + UnconnectedINPs(cb, sc) + InternalInputs(cb, sc);
+      ScInputBoundary(cb, sc);
+    }
+    assert ScInputBoundary(ca, sc) == ScInputBoundary(cb, sc);
+    //NPBetweenSubcircuitsComplement(c, sc, sc) + UnconnectedINPs(c, sc) + InternalInputs(c, sc)
+    assert (forall np: NP :: (np in ScInputBoundary(ca, sc)) == (np in ScInputBoundary(cb, sc)));
+    assert (forall np: NP :: (np !in ScInputBoundary(ca, sc)) && np.n in sc ==> (np in ca.PortSource) == (np in cb.PortSource));
+    assert (forall np: NP :: (np !in ScInputBoundary(ca, sc)) && np.n in sc && np in ca.PortSource ==> ca.PortSource[np] == cb.PortSource[np]);
+  }
+
+  ghost opaque predicate ConservedValid(ca: Circuit, cb: Circuit, e: Equiv, known: map<NP, bool>)
   {
     CircuitValid(ca) && CircuitValid(cb) &&
     EquivValid(ca, e) && EquivValid(cb, e) &&
@@ -50,21 +130,29 @@ module ConservedSubcircuit {
     requires forall np :: np in path ==> np.n in e.sc
     requires PathValid(ca, path)
     requires Seq.HasNoDuplicates(path)
-    requires INPValid(ca, path[|path|-1])
+    requires INPValid(ca, Seq.Last(path))
     ensures PathValid(cb, path)
     ensures
+      CircuitValid(ca) && CircuitValid(cb) &&
+      INPValid(cb, Seq.Last(path)) &&
       EvaluateINPInner(ca, path, knowns) == EvaluateINPInner(cb, path, knowns)
     decreases |NodesNotInPath(ca, path)|, 2
   {
+    reveal ConservedValid();
     reveal EquivValid();
-    var head := path[|path|-1];
-    var tail := path[..|path|-1];
+    reveal PathValid();
+    reveal CircuitValid();
+    reveal SubcircuitConserved();
+    var head := Seq.Last(path);
+    var tail := Seq.DropLast(path);
     if head in knowns {
+      assert EvaluateINPInner(ca, path, knowns) == EvaluateINPInner(cb, path, knowns);
     } else {
       if head in ca.PortSource {
         var onp := ca.PortSource[head];
         if onp in path {
         } else {
+          reveal CircuitValid();
           NodesNotInPathDecreases(ca, path, onp);
           StillHasNoDuplicates(path, onp);
           EvaluateONPInnerConserved(ca, cb, e, path + [onp], knowns);
@@ -78,19 +166,28 @@ module ConservedSubcircuit {
       ca: Circuit, cb: Circuit, e: Equiv, path: seq<NP>, knowns: map<NP, bool>)
     requires ConservedValid(ca, cb, e, knowns)
     requires |path| > 0
-    requires ONPValid(ca, path[|path|-1])
-    requires path[|path|-1] !in knowns
+    requires ONPValid(ca, Seq.Last(path))
+    requires Seq.Last(path) !in knowns
     requires forall np :: np in path ==> np.n in e.sc
     requires
-      var nk := ca.NodeKind[path[|path|-1].n];
+      var nk := ca.NodeKind[Seq.Last(path).n];
       nk.CXor? || nk.CAnd?
     requires PathValid(ca, path)
     requires Seq.HasNoDuplicates(path)
     ensures PathValid(cb, path)
-    ensures EvaluateONPBinary(ca, path, knowns) == EvaluateONPBinary(cb, path, knowns)
+    ensures
+      CircuitValid(ca) && CircuitValid(cb) &&
+      ONPValid(cb, Seq.Last(path)) &&
+      var nk := cb.NodeKind[Seq.Last(path).n];
+      (nk.CXor? || nk.CAnd?) &&
+      EvaluateONPBinary(ca, path, knowns) == EvaluateONPBinary(cb, path, knowns)
     decreases |NodesNotInPath(ca, path)|, 3
   {
+    reveal ConservedValid();
     reveal EquivValid();
+    reveal PathValid();
+    reveal CircuitValid();
+    reveal SubcircuitConserved();
     var nk := ca.NodeKind[path[|path|-1].n];
     var head := path[|path|-1];
     assert NodeValid(ca, head.n);
@@ -119,10 +216,19 @@ module ConservedSubcircuit {
     requires forall np :: np in path ==> np.n in e.sc
     requires Seq.HasNoDuplicates(path)
     ensures PathValid(cb, path)
-    ensures EvaluateONPUnary(ca, path, knowns) == EvaluateONPUnary(cb, path, knowns)
+    ensures
+      CircuitValid(ca) && CircuitValid(cb) &&
+      ONPValid(cb, Seq.Last(path)) &&
+      var nk := cb.NodeKind[Seq.Last(path).n];
+      nk.CInv? &&
+      EvaluateONPUnary(ca, path, knowns) == EvaluateONPUnary(cb, path, knowns)
     decreases |NodesNotInPath(ca, path)|, 3
   {
+    reveal ConservedValid();
     reveal EquivValid();
+    reveal PathValid();
+    reveal CircuitValid();
+    reveal SubcircuitConserved();
     var head := path[|path|-1];
     var inp_0 := NP(head.n, INPUT_0);
     if inp_0 in path {
@@ -139,10 +245,17 @@ module ConservedSubcircuit {
     requires EvaluateONPInnerRequirements(ca, path, knowns)
     requires forall np :: np in path ==> np.n in e.sc
     ensures PathValid(cb, path)
-    ensures EvaluateONPInner(ca, path, knowns) == EvaluateONPInner(cb, path, knowns)
+    ensures
+      CircuitValid(ca) && CircuitValid(cb) &&
+      ONPValid(cb, Seq.Last(path)) &&
+      EvaluateONPInner(ca, path, knowns) == EvaluateONPInner(cb, path, knowns)
     decreases |NodesNotInPath(ca, path)|, 4
   {
+    reveal ConservedValid();
     reveal EquivValid();
+    reveal PathValid();
+    reveal CircuitValid();
+    reveal SubcircuitConserved();
     var head := path[|path|-1];
     if head in knowns {
     } else {
@@ -162,9 +275,15 @@ module ConservedSubcircuit {
     requires o.n in e.sc
     requires INPValid(ca, o) || ONPValid(ca, o)
     ensures INPValid(cb, o) || ONPValid(cb, o)
-    ensures Evaluate(ca, o, known) == Evaluate(cb, o, known)
+    ensures
+      CircuitValid(ca) && CircuitValid(cb) &&
+      (Evaluate(ca, o, known) == Evaluate(cb, o, known))
   {
+    reveal ConservedValid();
     reveal EquivValid();
+    reveal PathValid();
+    reveal CircuitValid();
+    reveal SubcircuitConserved();
     assert PathValid(ca, [o]);
     LengthOneNoDuplicates([o]);
     if INPValid(ca, o) {
@@ -174,16 +293,75 @@ module ConservedSubcircuit {
     }
   }
 
+  lemma ScInputBoundaryConserved(ca: Circuit, cb: Circuit, e: Equiv)
+    requires CircuitValid(ca)
+    requires CircuitValid(cb)
+    requires CircuitConserved(ca, cb)
+    requires forall n :: n in e.sc ==> n in ca.NodeKind
+  {
+    assert CircuitValid(ca);
+    reveal CircuitValid();
+    reveal CircuitConserved();
+    reveal ScValid();
+  }
+
+  lemma ScOutputBoundaryConserved(ca: Circuit, cb: Circuit, e: Equiv)
+    requires CircuitValid(ca)
+    requires CircuitValid(cb)
+    requires CircuitConserved(ca, cb)
+    requires CircuitUnconnected(ca, cb)
+    requires EquivValid(ca, e)
+    ensures ScOutputBoundary(ca, e.sc) == ScOutputBoundary(cb, e.sc)
+  {
+    reveal CircuitValid();
+    reveal CircuitConserved();
+    reveal CircuitUnconnected();
+    reveal EquivValid();
+    reveal EquivScOutputsInOutputs();
+    reveal ScValid();
+  }
+
+
+  lemma EquivConserved2(ca: Circuit, cb: Circuit, e: Equiv)
+    requires CircuitValid(ca)
+    requires CircuitValid(cb)
+    requires CircuitConserved(ca, cb)
+    requires CircuitUnconnected(ca, cb)
+    requires EquivValid(ca, e)
+    ensures EquivValid(cb, e)
+    ensures EquivValid(ca, e) ==> EquivTrue(ca, e) == EquivTrue(cb, e)
+  {
+    reveal EquivValid();
+    CircuitConservedToSubcircuitConserved(ca, cb, e.sc);
+    assert EquivScOutputsInOutputs(ca, e.sc, e.outputs);
+    reveal EquivScOutputsInOutputs();
+    reveal CircuitConserved();
+    reveal CircuitUnconnected();
+    reveal ScValid();
+    EquivConserved(ca, cb, e);
+  }
+
   lemma EquivConserved(ca: Circuit, cb: Circuit, e: Equiv)
     requires CircuitValid(ca)
     requires CircuitValid(cb)
     requires SubcircuitConserved(ca, cb, e.sc)
-    requires forall np :: np in ScOutputBoundary(ca, e.sc) ==> np in e.outputs
-    requires forall np :: np in ScOutputBoundary(cb, e.sc) ==> np in e.outputs
+    requires EquivScOutputsInOutputs(ca, e.sc, e.outputs)
+    requires EquivScOutputsInOutputs(cb, e.sc, e.outputs)
     ensures EquivValid(ca, e) == EquivValid(cb, e)
     ensures EquivValid(ca, e) ==> EquivTrue(ca, e) == EquivTrue(cb, e)
   {
+    reveal EquivScOutputsInOutputs();
+    reveal CircuitValid();
     reveal EquivValid();
+    reveal EquivTrue();
+    reveal ConservedValid();
+
+    reveal ScValid();
+    reveal NPsValidAndInSc();
+    reveal SubcircuitConserved();
+
+    assert ScValid(ca, e.sc) == ScValid(cb, e.sc);
+
     assert EquivValid(ca, e) == EquivValid(cb, e);
     if EquivValid(ca, e) {
       forall knowns: map<NP, bool> | knowns.Keys == e.inputs
