Attempt2/Equiv.dfy
@@ -27,31 +27,42 @@ module Equiv {
 
   function SwapEquivF(c: Circuit, e: Equiv, f: map<NP, bool> --> map<NP, bool>): (r: Equiv)
     requires EquivValid(c, e)
-    requires (forall knowns: map<NP, bool> :: (knowns.Keys == e.inputs) ==> f.requires(knowns))
-    requires (forall knowns: map<NP, bool> :: (knowns.Keys == e.inputs) ==> f(knowns).Keys == e.outputs)
+    requires MapFunctionValid(MapFunction(e.inputs, e.outputs, f))
     ensures EquivValid(c, r)
   {
     reveal EquivValid();
     Equiv(e.sc, e.inputs, e.outputs, f)
   }
 
-  ghost opaque predicate EquivValid(c: Circuit, e: Equiv)
+  opaque predicate NPsValidAndInSc(c: Circuit, sc: set<CNode>, nps: set<NP>)
   {
-    ScValid(c, e.sc) &&
-    (ScInputBoundary(c, e.sc) == e.inputs) &&
-    SetsNoIntersection(e.inputs, e.outputs) &&
-    (forall np :: np in e.outputs ==> (INPValid(c, np) || ONPValid(c, np)) && np.n in e.sc) &&
-    (forall knowns: map<NP, bool> :: (knowns.Keys == e.inputs) ==> e.f.requires(knowns)) &&
-    (forall knowns: map<NP, bool> :: (knowns.Keys == e.inputs) ==> e.f(knowns).Keys == e.outputs) &&
-    // But it is possible to have outputs that are not on output boundary (i.e. we plan to connect them in the future)
-    (forall np :: np in ScOutputBoundary(c, e.sc) ==> np in e.outputs)
+    (forall np :: np in nps ==> NPValid(c, np) && np.n in sc)
   }
 
-  ghost predicate EquivTrue(c: Circuit, e: Equiv)
+  opaque predicate EquivScOutputsInOutputs(c: Circuit, sc: set<CNode>, outputs: set<NP>)
+  {
+    (forall np :: np in ScOutputBoundary(c, sc) ==> np in outputs)
+  }
+
+  ghost opaque predicate EquivValid(c: Circuit, e: Equiv)
+  {
+    && ScValid(c, e.sc)
+    && (ScInputBoundary(c, e.sc) == e.inputs)
+    && SetsNoIntersection(e.inputs, e.outputs)
+    && NPsValidAndInSc(c, e.sc, e.outputs)
+    && NPsValidAndInSc(c, e.sc, e.inputs)
+    && MapFunctionValid(EtoMf(e))
+    && EquivScOutputsInOutputs(c, e.sc, e.outputs)
+  }
+
+  ghost opaque predicate EquivTrue(c: Circuit, e: Equiv)
     requires CircuitValid(c)
     requires EquivValid(c, e)
   {
+    reveal CircuitValid();
     reveal EquivValid();
+    reveal MapFunctionValid();
+    reveal NPsValidAndInSc();
     forall knowns: map<NP, bool> :: (knowns.Keys == e.inputs) ==>
       forall np :: np in e.outputs ==>
         Evaluate(c, np, knowns) == EvalOk(e.f(knowns)[np])
