Attempt2/Build/And.dfy
@@ -3,6 +3,9 @@ module Build.And {
   import opened Circ
   import opened Equiv
   import opened Eval
+  import opened Utils
+  import opened MapFunction
+  import opened ConservedSubcircuit
 
   datatype AndPorts = AndPorts(
     i_0: NP,
@@ -23,10 +26,9 @@ module Build.And {
     ensures EquivValid(r.0, r.2)
   {
     reveal EquivValid();
+    reveal CircuitValid();
     var new_node := GetNewNode(c);
     assert new_node !in c.NodeKind;
-    //assert forall np: NP :: np in c.PortSource.Keys ==> np.n != new_node;
-    //assert forall np: NP :: np in c.PortSource.Values ==> np.n != new_node;
     var new_c := Circuit(
       NodeKind := c.NodeKind[new_node := CAnd],
       PortSource := c.PortSource
@@ -40,7 +42,12 @@ module Build.And {
     var f: map<NP, bool> --> map<NP, bool> := (x: map<NP, bool>) requires x.Keys == inputs =>
       AndBehav(m, x);
     var e := Equiv({new_node}, inputs, outputs, f);
-    //assert ScOutputBoundary(new_c, e.sc) == {};
+    assert forall np :: np in new_c.PortSource.Values ==> np.n !in e.sc;
+    reveal ScValid();
+    reveal NPsValidAndInSc();
+    reveal EquivScOutputsInOutputs();
+    reveal MapFunctionValid();
+    assert EquivValid(new_c, e);
     (new_c, m, e)
   }
 
@@ -48,10 +55,14 @@ module Build.And {
     requires CircuitValid(c)
     ensures
       var (new_c, m, e) := InsertAndImpl(c);
-      EquivTrue(new_c, e)
+      && EquivValid(new_c, e)
+      && EquivTrue(new_c, e)
   {
     var (new_c, m, e) := InsertAndImpl(c);
     var path := [m.o];
+    assert PathValid(new_c, path) && PathValid(new_c, [m.o, m.i_0]) && PathValid(new_c, [m.o, m.i_1]) by {
+      reveal PathValid();
+    }
     LengthOneNoDuplicates(path);
     assert CircuitValid(new_c);
     forall knowns: map<NP, bool> | knowns.Keys == e.inputs
@@ -73,17 +84,42 @@ module Build.And {
       assert Evaluate(new_c, m.o, knowns) == EvalOk(iv_0 && iv_1);
       assert Evaluate(new_c, m.o, knowns) == EvalOk(e.f(knowns)[m.o]);
     }
+    reveal EquivTrue();
     assert EquivTrue(new_c, e);
+  }
+
+  lemma InsertAndConserves(c: Circuit)
+    requires CircuitValid(c)
+    ensures CircuitConserved(c, InsertAndImpl(c).0)
+    ensures CircuitUnconnected(c, InsertAndImpl(c).0)
+    ensures
+      var (new_c, m, e) := InsertAndImpl(c);
+      SubcircuitIsIsland(new_c, e.sc)
+  {
+    reveal CircuitConserved();
+    reveal CircuitUnconnected();
+    var (new_c, m, e) := InsertAndImpl(c);
+    reveal CircuitValid();
+    assert (forall np :: np in c.PortSource.Keys ==> np.n !in e.sc);
+    assert (forall np :: np in c.PortSource.Values ==> np.n !in e.sc);
+    assert (forall np :: np in new_c.PortSource && np.n in e.sc ==> new_c.PortSource[np].n in e.sc);
+    assert (forall np :: np in new_c.PortSource && np.n !in e.sc ==> new_c.PortSource[np].n !in e.sc);
+    reveal SubcircuitIsIsland();
   }
 
   function InsertAnd(c: Circuit): (r: (Circuit, AndPorts, Equiv))
     requires CircuitValid(c)
     ensures
       var (new_c, m, e) := r;
-      r == InsertAndImpl(c) &&
-      EquivTrue(new_c, e)
+      && r == InsertAndImpl(c)
+      && CircuitValid(r.0)
+      && EquivTrue(new_c, e)
+      && CircuitConserved(c, r.0)
+      && CircuitUnconnected(c, r.0)
+      && SubcircuitIsIsland(new_c, e.sc)
   {
     InsertAndCorrect(c);
+    InsertAndConserves(c);
     InsertAndImpl(c)
   }
 
@@ -94,6 +130,7 @@ module Build.And {
       ScOutputBoundary(new_c, e.sc) == {}
   {
     var (new_c, p, e) := InsertAnd(c);
+    reveal CircuitValid();
     assert forall np: NP :: np.n in e.sc ==> np !in c.PortSource.Values;
   }
 
