Attempt2/ComposeEval.dfy
@@ -12,33 +12,94 @@ module ComposeEval {
   lemma NPNotInPathHelper(np: NP, sc1: set<CNode>, sc2: set<CNode>, prepath: seq<NP>, path: seq<NP>)
     requires np.n in sc1
     requires SetsNoIntersection(sc1, sc2)
-    requires forall np :: np in prepath ==> np.n in sc2
-    requires forall np :: np in path ==> np.n in sc1
+    requires PathInSubcircuit(prepath, sc2)
+    requires PathInSubcircuit(path, sc1)
     ensures (np in path) == (np in (prepath + path))
   {
+    reveal PathInSubcircuit();
+    if np.n in sc2 {
+      assert np.n in sc1 * sc2;
+    }
+    assert np.n !in sc2;
+    assert np !in prepath;
   }
-  
-  lemma {:vcs_split_on_every_assert} EvaluateONPBinaryComposed1(
+
+  opaque predicate PathInSubcircuit(path: seq<NP>, sc: set<CNode>)
+  {
+    forall np :: np in path ==> np.n in sc
+  }
+
+  lemma EvaluateONPComposed1Helper(
+      c: Circuit, e1: Equiv, e2: Equiv, prepath: seq<NP>, path: seq<NP>, knowns: map<NP, bool>, inp: NP)
+    requires CircuitValid(c)
+    requires ComposedValid(c, e1, e2)
+    requires GoodKnownKeys(c, e1, e2, knowns)
+    requires PathInSubcircuit(prepath, e2.sc)
+    requires PathInSubcircuit(path, e1.sc)
+    requires EvaluateONPUnaryBinaryRequirements(c, path, knowns)
+    requires EvaluateONPUnaryBinaryRequirements(c, prepath + path, knowns)
+    requires INPValid(c, inp)
+    requires inp !in path
+    requires inp.n in e1.sc
+    ensures
+      (forall np :: np in e1.inputs ==> np in knowns) &&
+      var knowns_1 := ExtractMap(knowns, e1.inputs);
+      var new_path := path + [inp];
+      Seq.HasNoDuplicates(new_path) &&
+      Seq.HasNoDuplicates(prepath + new_path) &&
+      PathValid(c, new_path) &&
+      PathValid(c, prepath + new_path) &&
+      EvaluateINPInner(c, new_path, knowns) == EvaluateINPInner(c, new_path, knowns_1) &&
+      Simpl(EvaluateINPInner(c, new_path, knowns)) == Simpl(EvaluateINPInner(c, prepath+new_path, knowns))
+    decreases |NodesNotInPath(c, prepath + path)|, 3
+  {
+    StillHasNoDuplicates(path, inp);
+    assert inp !in prepath by {
+      reveal PathInSubcircuit();
+      reveal ComposedValid();
+      InThisNotInThat(inp.n, e1.sc, e2.sc);
+    }
+    StillHasNoDuplicates(prepath + path, inp);
+    AppendPathValid(c, path, inp);
+    AppendPathValid(c, prepath + path, inp);
+    assert forall np :: np in e1.inputs ==> np in knowns by {reveal GoodKnownKeys();}
+    var knowns_1 := ExtractMap(knowns, e1.inputs);
+    var new_path := path + [inp];
+    NodesNotInPathDecreases(c, prepath + path, inp);
+    assert PathInSubcircuit(new_path, e1.sc) by {reveal PathInSubcircuit();}
+    assert (prepath + path) + [inp] == prepath + (path + [inp]);
+    assert Seq.Last(prepath + new_path) == inp;
+    EvaluateINPInnerComposed1(c, e1, e2, prepath, new_path, knowns);
+    assert EvaluateINPInner(c, new_path, knowns) == EvaluateINPInner(c, new_path, knowns_1);
+    assert Simpl(EvaluateINPInner(c, new_path, knowns)) == Simpl(EvaluateINPInner(c, prepath+new_path, knowns));
+  }
+
+  lemma EvaluateONPBinaryComposed1(
       c: Circuit, e1: Equiv, e2: Equiv, prepath: seq<NP>, path: seq<NP>, knowns: map<NP, bool>)
     requires CircuitValid(c)
     requires ComposedValid(c, e1, e2)
-    requires knowns.Keys == ComposeEquivInputs(c, e1, e2)
-    requires forall np :: np in prepath ==> np.n in e2.sc
-    requires forall np :: np in path ==> np.n in e1.sc
+    requires GoodKnownKeys(c, e1, e2, knowns)
+    requires PathInSubcircuit(prepath, e2.sc)
+    requires PathInSubcircuit(path, e1.sc)
     requires EvaluateONPBinaryRequirements(c, path, knowns)
     requires EvaluateONPBinaryRequirements(c, prepath + path, knowns)
     ensures
+      (forall np :: np in e1.inputs ==> np in knowns) &&
       var knowns_1 := ExtractMap(knowns, e1.inputs);
       var np := Seq.Last(path);
       (EvaluateONPBinary(c, path, knowns) == EvaluateONPBinary(c, path, knowns_1)) &&
       (Simpl(EvaluateONPBinary(c, path, knowns)) == Simpl(EvaluateONPBinary(c, prepath+path, knowns)))
-    decreases |NodesNotInPath(c, prepath + path)|, 3
+    decreases |NodesNotInPath(c, prepath + path)|, 4
   {
+    assert forall np :: np in e1.inputs ==> np in knowns by {reveal GoodKnownKeys();}
     var knowns_1 := ExtractMap(knowns, e1.inputs);
     var head := Seq.Last(path);
+    assert head == Seq.Last(prepath + path);
+    assert head.n in e1.sc by {reveal PathInSubcircuit();}
     assert NodeValid(c, head.n);
     var inp_0 := NP(head.n, INPUT_0);
     var inp_1 := NP(head.n, INPUT_1);
+    assert INPValid(c, inp_0) && INPValid(c, inp_1) by {reveal CircuitValid();}
     SetsNoIntersectionFromComposedValid(c, e1, e2);
     NPNotInPathHelper(inp_0, e1.sc, e2.sc, prepath, path);
     NPNotInPathHelper(inp_1, e1.sc, e2.sc, prepath, path);
@@ -49,103 +110,157 @@ module ComposeEval {
       assert (EvaluateONPBinary(c, path, knowns) == EvaluateONPBinary(c, path, knowns_1));
       assert (Simpl(EvaluateONPBinary(c, path, knowns)) == Simpl(EvaluateONPBinary(c, prepath+path, knowns)));
     } else {
-      NodesNotInPathDecreases(c, prepath + path, inp_0);
-      NodesNotInPathDecreases(c, prepath + path, inp_1);
-      StillHasNoDuplicates(path, inp_0);
-      StillHasNoDuplicates(prepath + path, inp_0);
-      assert (prepath + path) + [inp_0] == prepath + (path + [inp_0]);
-      assert Seq.HasNoDuplicates(prepath + (path + [inp_0]));
-      StillHasNoDuplicates(path, inp_1);
-      StillHasNoDuplicates(prepath + path, inp_1);
-      assert (prepath + path) + [inp_1] == prepath + (path + [inp_1]);
-      assert Seq.HasNoDuplicates(prepath + (path + [inp_1]));
-      EvaluateINPInnerComposed1(c, e1, e2, prepath, path + [inp_0], knowns);
-      EvaluateINPInnerComposed1(c, e1, e2, prepath, path + [inp_1], knowns);
-      assert (EvaluateONPBinary(c, path, knowns) == EvaluateONPBinary(c, path, knowns_1));
+      EvaluateONPComposed1Helper(c, e1, e2, prepath, path, knowns, inp_0);
+      EvaluateONPComposed1Helper(c, e1, e2, prepath, path, knowns, inp_1);
+
+      assert prepath + (path + [inp_0]) == (prepath + path) + [inp_0];
+      assert prepath + (path + [inp_1]) == (prepath + path) + [inp_1];
+
       assert (Simpl(EvaluateONPBinary(c, path, knowns)) == Simpl(EvaluateONPBinary(c, prepath+path, knowns)));
     }
   }
 
-  lemma {:vcs_split_on_every_assert} EvaluateONPBinaryComposed2(
+  lemma EvaluateONPComposed2Helper(
+      c: Circuit, e1: Equiv, e2: Equiv, path: seq<NP>, knowns: map<NP, bool>, inp: NP)
+    requires CircuitValid(c)
+    requires ComposedValid(c, e1, e2)
+    requires GoodKnownKeys(c, e1, e2, knowns)
+    requires PathInSubcircuit(path, e2.sc)
+    requires EvaluateONPUnaryBinaryRequirements(c, path, knowns)
+    requires INPValid(c, inp)
+    requires inp !in path
+    requires inp.n in e2.sc
+    ensures
+      var knowns_2 := CalculateE2Inputs(c, e1, e2, knowns);
+      var new_path := path + [inp];
+      Seq.HasNoDuplicates(new_path) &&
+      PathValid(c, new_path) &&
+      (EvaluateINPInner(c, new_path, knowns) == EvaluateINPInner(c, new_path, knowns_2))
+    decreases |NodesNotInPath(c, path)|, 4
+  {
+    StillHasNoDuplicates(path, inp);
+    AppendPathValid(c, path, inp);
+    var knowns_2 := CalculateE2Inputs(c, e1, e2, knowns);
+    var new_path := path + [inp];
+    NodesNotInPathDecreases(c, path, inp);
+    reveal PathInSubcircuit();
+    EvaluateINPInnerComposed2(c, e1, e2, new_path, knowns);
+    assert (EvaluateINPInner(c, new_path, knowns) == EvaluateINPInner(c, new_path, knowns_2));
+  }
+
+  lemma EvaluateONPBinaryComposed2(
       c: Circuit, e1: Equiv, e2: Equiv, path: seq<NP>, knowns: map<NP, bool>)
     requires CircuitValid(c)
     requires ComposedValid(c, e1, e2)
-    requires knowns.Keys == ComposeEquivInputs(c, e1, e2)
-    requires forall np :: np in path ==> np.n in e2.sc
+    requires GoodKnownKeys(c, e1, e2, knowns)
+    requires PathInSubcircuit(path, e2.sc)
     requires EvaluateONPBinaryRequirements(c, path, knowns)
     ensures
       var knowns_2 := CalculateE2Inputs(c, e1, e2, knowns);
-      var np := Seq.Last(path);
+      (Seq.Last(path) !in knowns_2) &&
       (EvaluateONPBinary(c, path, knowns) == EvaluateONPBinary(c, path, knowns_2))
-    decreases |NodesNotInPath(c, path)|, 3
+    decreases |NodesNotInPath(c, path)|, 5
   {
-    var nk := c.NodeKind[path[|path|-1].n];
-    var head := path[|path|-1];
+    var head := Seq.Last(path);
+    assert head.n in e2.sc by {
+      reveal PathInSubcircuit();
+    }
+    var nk := c.NodeKind[head.n];
     assert NodeValid(c, head.n);
     var inp_0 := NP(head.n, INPUT_0);
     var inp_1 := NP(head.n, INPUT_1);
+    assert INPValid(c, inp_0) && INPValid(c, inp_1) by {reveal CircuitValid();}
+    var knowns_2 := CalculateE2Inputs(c, e1, e2, knowns);
+    assert head !in knowns;
+    ONPNotInKnownsNotInKnowns2(c, head, e1, e2, knowns);
+    assert head !in knowns_2;
     if inp_0 in path {
+      assert (EvaluateONPBinary(c, path, knowns) == EvaluateONPBinary(c, path, knowns_2));
     } else if inp_1 in path {
+      assert (EvaluateONPBinary(c, path, knowns) == EvaluateONPBinary(c, path, knowns_2));
     } else {
-      NodesNotInPathDecreases(c, path, inp_0);
-      NodesNotInPathDecreases(c, path, inp_1);
-      StillHasNoDuplicates(path, inp_0);
-      StillHasNoDuplicates(path, inp_1);
-      EvaluateINPInnerComposed2(c, e1, e2, path + [inp_0], knowns);
-      EvaluateINPInnerComposed2(c, e1, e2, path + [inp_1], knowns);
+      assert 
+        var new_path := path + [inp_0];
+        Seq.HasNoDuplicates(new_path) &&
+        PathValid(c, new_path) &&
+        (EvaluateINPInner(c, new_path, knowns) == EvaluateINPInner(c, new_path, knowns_2)) by {
+          EvaluateONPComposed2Helper(c, e1, e2, path, knowns, inp_0);
+        }
+      assert 
+        var new_path := path + [inp_1];
+        Seq.HasNoDuplicates(new_path) &&
+        PathValid(c, new_path) &&
+        (EvaluateINPInner(c, new_path, knowns) == EvaluateINPInner(c, new_path, knowns_2)) by {
+          EvaluateONPComposed2Helper(c, e1, e2, path, knowns, inp_1);
+        }
+      assert EvaluateONPBinary(c, path, knowns) == EvaluateONPBinary(c, path, knowns_2);
     }
+    assert
+      var knowns_2 := CalculateE2Inputs(c, e1, e2, knowns);
+      (EvaluateONPBinary(c, path, knowns) == EvaluateONPBinary(c, path, knowns_2));
   }
 
-  lemma {:vcs_split_on_every_assert} EvaluateONPUnaryComposed1(
+  lemma EvaluateONPUnaryComposed1(
       c: Circuit, e1: Equiv, e2: Equiv, prepath: seq<NP>, path: seq<NP>, knowns: map<NP, bool>)
     requires CircuitValid(c)
     requires ComposedValid(c, e1, e2)
-    requires knowns.Keys == ComposeEquivInputs(c, e1, e2)
-    requires forall np :: np in prepath ==> np.n in e2.sc
-    requires forall np :: np in path ==> np.n in e1.sc
+    requires GoodKnownKeys(c, e1, e2, knowns)
+    requires PathInSubcircuit(prepath, e2.sc)
+    requires PathInSubcircuit(path, e1.sc)
     requires EvaluateONPUnaryRequirements(c, path, knowns)
     requires EvaluateONPUnaryRequirements(c, prepath+path, knowns)
     ensures
+      (forall np :: np in e1.inputs ==> np in knowns) &&
       var knowns_1 := ExtractMap(knowns, e1.inputs);
       var np := Seq.Last(path);
       (EvaluateONPUnary(c, path, knowns) == EvaluateONPUnary(c, path, knowns_1)) &&
       (Simpl(EvaluateONPUnary(c, path, knowns)) == Simpl(EvaluateONPUnary(c, prepath+path, knowns)))
-    decreases |NodesNotInPath(c, prepath + path)|, 3
+    decreases |NodesNotInPath(c, prepath + path)|, 5
   {
-    var head := path[|path|-1];
+    assert forall np :: np in e1.inputs ==> np in knowns by {reveal GoodKnownKeys();}
+    var knowns_1 := ExtractMap(knowns, e1.inputs);
+    var head := Seq.Last(path);
+    assert head == Seq.Last(prepath + path);
+    assert head.n in e1.sc by {reveal PathInSubcircuit();}
+    assert NodeValid(c, head.n);
     var inp_0 := NP(head.n, INPUT_0);
+    assert INPValid(c, inp_0) by {reveal CircuitValid();}
     SetsNoIntersectionFromComposedValid(c, e1, e2);
     NPNotInPathHelper(inp_0, e1.sc, e2.sc, prepath, path);
     if inp_0 in path {
+      assert (EvaluateONPUnary(c, path, knowns) == EvaluateONPUnary(c, path, knowns_1));
+      assert (Simpl(EvaluateONPUnary(c, path, knowns)) == Simpl(EvaluateONPUnary(c, prepath+path, knowns)));
     } else {
-      NodesNotInPathDecreases(c, prepath + path, inp_0);
-      StillHasNoDuplicates(path, inp_0);
-      StillHasNoDuplicates(prepath + path, inp_0);
-      assert (prepath + path) + [inp_0] == prepath + (path + [inp_0]);
-      assert Seq.HasNoDuplicates(prepath + (path + [inp_0]));
-      EvaluateINPInnerComposed1(c, e1, e2, prepath, path + [inp_0], knowns);
+      EvaluateONPComposed1Helper(c, e1, e2, prepath, path, knowns, inp_0);
+      assert prepath + (path + [inp_0]) == (prepath + path) + [inp_0];
+      assert (Simpl(EvaluateONPUnary(c, path, knowns)) == Simpl(EvaluateONPUnary(c, prepath+path, knowns)));
     }
   }
 
-  lemma {:vcs_split_on_every_assert} EvaluateONPUnaryComposed2(
+  lemma EvaluateONPUnaryComposed2(
       c: Circuit, e1: Equiv, e2: Equiv, path: seq<NP>, knowns: map<NP, bool>)
     requires CircuitValid(c)
     requires ComposedValid(c, e1, e2)
-    requires knowns.Keys == ComposeEquivInputs(c, e1, e2)
-    requires forall np :: np in path ==> np.n in e2.sc
+    requires GoodKnownKeys(c, e1, e2, knowns)
+    requires PathInSubcircuit(path, e2.sc)
     requires EvaluateONPUnaryRequirements(c, path, knowns)
     ensures
       var knowns_2 := CalculateE2Inputs(c, e1, e2, knowns);
-      var np := Seq.Last(path);
+      (Seq.Last(path) !in knowns_2) &&
       EvaluateONPUnary(c, path, knowns) == EvaluateONPUnary(c, path, knowns_2)
-    decreases |NodesNotInPath(c, path)|, 3
+    decreases |NodesNotInPath(c, path)|, 4
   {
-    var head := path[|path|-1];
+    var head := Seq.Last(path);
+    assert head !in knowns;
+    ONPNotInKnownsNotInKnowns2(c, head, e1, e2, knowns);
     var inp_0 := NP(head.n, INPUT_0);
     if inp_0 in path {
     } else {
       NodesNotInPathDecreases(c, path, inp_0);
       StillHasNoDuplicates(path, inp_0);
+      assert PathInSubcircuit(path + [inp_0], e2.sc) by {
+        reveal PathInSubcircuit();
+      }
       EvaluateINPInnerComposed2(c, e1, e2, path + [inp_0], knowns);
     }
   }
@@ -161,47 +276,82 @@ module ComposeEval {
     reveal Seq.HasNoDuplicates();
   }
 
-  lemma {:vcs_split_on_every_assert} EvaluateINPInnerComposed1(c: Circuit, e1: Equiv, e2: Equiv, prepath: seq<NP>, path: seq<NP>, knowns: map<NP, bool>)
+  lemma EvaluateINPInnerComposed1(c: Circuit, e1: Equiv, e2: Equiv, prepath: seq<NP>, path: seq<NP>, knowns: map<NP, bool>)
     requires CircuitValid(c)
     requires ComposedValid(c, e1, e2)
-    requires knowns.Keys == ComposeEquivInputs(c, e1, e2)
-    requires forall np :: np in path ==> np.n in e1.sc
-    requires forall np :: np in prepath ==> np.n in e2.sc
+    requires GoodKnownKeys(c, e1, e2, knowns)
+    requires PathInSubcircuit(path, e1.sc)
+    requires PathInSubcircuit(prepath, e2.sc)
     requires EvaluateINPInnerRequirements(c, path, knowns)
     requires EvaluateINPInnerRequirements(c, prepath + path, knowns)
     ensures
+      (forall np :: np in e1.inputs ==> np in knowns) &&
       var knowns_1 := ExtractMap(knowns, e1.inputs);
-      var knowns_2 := CalculateE2Inputs(c, e1, e2, knowns);
-      var np := Seq.Last(path);
       (EvaluateINPInner(c, path, knowns) == EvaluateINPInner(c, path, knowns_1)) &&
       (Simpl(EvaluateINPInner(c, path, knowns)) == Simpl(EvaluateINPInner(c, prepath+path, knowns)))
     decreases |NodesNotInPath(c, prepath + path)|, 2
   {
-    reveal ComposedValid();
-    reveal EquivValid();
+    assert forall np :: np in e1.inputs ==> np in knowns by {reveal GoodKnownKeys();}
     var knowns_1 := ExtractMap(knowns, e1.inputs);
     var knowns_2 := CalculateE2Inputs(c, e1, e2, knowns);
     var np := Seq.Last(path);
+    assert np.n in e1.sc by {
+      reveal PathInSubcircuit();
+    }
     var tail := Seq.DropLast(path);
     assert Seq.HasNoDuplicates(path);
     HasNoDuplicatesMeansHeadNotInTail(path);
     assert np !in tail;
     if np in e1.inputs {
+      assert np in knowns;
+      assert np in knowns_1;
       assert EvaluateINPInner(c, path, knowns) == EvaluateINPInner(c, path, knowns_1);
       assert Simpl(EvaluateINPInner(c, path, knowns)) == Simpl(EvaluateINPInner(c, prepath+path, knowns));
     } else {
+      assert np !in knowns by {
+        reveal ComposedValid();
+        reveal ScValid();
+        reveal GoodKnownKeys();
+        assert knowns.Keys == (e1.inputs + e2.inputs) - NPBetweenSubcircuits(c, e2.sc, e1.sc);
+        InThisNotInThat(np.n, e1.sc, e2.sc);
+        assert np.n !in e2.sc;
+        reveal EquivValid();
+        assert np !in e2.inputs;
+      }
+      assert np !in knowns_1;
       if np in c.PortSource {
         var onp := c.PortSource[np];
-        assert onp.n in e1.sc;
+        assert ONPValid(c, onp) by {
+          reveal CircuitValid();
+        }
+        assert onp.n in e1.sc by {
+          reveal ComposedValid();
+          reveal EquivValid();
+          reveal PathInSubcircuit();
+        }
+        assert EvaluateINPInnerRequirements(c, path, knowns);
+        assert EvaluateINPInnerRequirements(c, path, knowns_1);
+        assert EvaluateINPInnerRequirements(c, prepath + path, knowns);
         if onp in path {
+          assert EvaluateINPInner(c, path, knowns) == EvalError({}, {path + [onp]});
           assert EvaluateINPInner(c, path, knowns) == EvaluateINPInner(c, path, knowns_1);
           assert Simpl(EvaluateINPInner(c, path, knowns)) == Simpl(EvaluateINPInner(c, prepath+path, knowns));
         } else {
+          assert NPValid(c, onp) by {
+            reveal CircuitValid();
+          }
+          SetsNoIntersectionFromComposedValid(c, e1, e2);
+          NPNotInPathHelper(onp, e1.sc, e2.sc, prepath, path);
           NodesNotInPathDecreases(c, prepath+path, onp);
           StillHasNoDuplicates(path, onp);
           StillHasNoDuplicates(prepath + path, onp);
+          AppendPathValid(c, path, onp);
+          AppendPathValid(c, prepath + path, onp);
           assert (prepath + path) + [onp] == prepath + (path + [onp]);
           assert Seq.HasNoDuplicates(prepath + (path + [onp]));
+          assert PathInSubcircuit(path + [onp], e1.sc) by {
+            reveal PathInSubcircuit();
+          }
           EvaluateONPInnerComposed1(c, e1, e2, prepath, path + [onp], knowns);
           assert EvaluateINPInner(c, path, knowns) == EvaluateINPInner(c, path, knowns_1);
           assert Simpl(EvaluateINPInner(c, path, knowns)) == Simpl(EvaluateINPInner(c, prepath+path, knowns));
@@ -213,24 +363,24 @@ module ComposeEval {
     }
   }
 
-  lemma {:vcs_split_on_every_assert} EvaluateINPInnerComposed2(c: Circuit, e1: Equiv, e2: Equiv, path: seq<NP>, knowns: map<NP, bool>)
+  lemma EvaluateINPInnerComposed2(c: Circuit, e1: Equiv, e2: Equiv, path: seq<NP>, knowns: map<NP, bool>)
     requires CircuitValid(c)
     requires ComposedValid(c, e1, e2)
-    requires knowns.Keys == ComposeEquivInputs(c, e1, e2)
-    requires forall np :: np in path ==> np.n in e2.sc
+    requires GoodKnownKeys(c, e1, e2, knowns)
+    requires PathInSubcircuit(path, e2.sc)
     requires EvaluateINPInnerRequirements(c, path, knowns)
     ensures
-      var knowns_1 := ExtractMap(knowns, e1.inputs);
       var knowns_2 := CalculateE2Inputs(c, e1, e2, knowns);
-      var np := Seq.Last(path);
       (EvaluateINPInner(c, path, knowns) == EvaluateINPInner(c, path, knowns_2))
     decreases |NodesNotInPath(c, path)|, 2
   {
-    reveal ComposedValid();
-    reveal EquivValid();
+    assert forall np :: np in e1.inputs ==> np in knowns by {reveal GoodKnownKeys();}
     var knowns_1 := ExtractMap(knowns, e1.inputs);
     var knowns_2 := CalculateE2Inputs(c, e1, e2, knowns);
     var np := Seq.Last(path);
+    assert np.n in e2.sc by {
+      reveal PathInSubcircuit();
+    }
     var tail := Seq.DropLast(path);
     assert Seq.HasNoDuplicates(path);
     HasNoDuplicatesMeansHeadNotInTail(path);
@@ -239,18 +389,51 @@ module ComposeEval {
       if np in knowns {
         assert EvaluateINPInner(c, path, knowns) == EvaluateINPInner(c, path, knowns_2);
       } else {
+        assert (np in c.PortSource) && (c.PortSource[np].n in e1.sc) by {
+          reveal GoodKnownKeys();
+          reveal ComposedValid();
+          assert knowns.Keys == (e1.inputs + e2.inputs) - NPBetweenSubcircuits(c, e2.sc, e1.sc);
+          assert np in NPBetweenSubcircuits(c, e2.sc, e1.sc);
+          assert c.PortSource[np].n in e1.sc;
+        }
         var onp := c.PortSource[np];
+        assert ONPValid(c, onp) by {
+          reveal CircuitValid();
+        }
         assert onp.n in e1.sc;
-        assert onp !in path;
+        assert onp !in path by {
+          reveal PathInSubcircuit();
+          reveal ComposedValid();
+          InThisNotInThat(onp.n, e1.sc, e2.sc);
+        } 
         NodesNotInPathDecreases(c, path, onp);
         StillHasNoDuplicates(path, onp);
         LengthOneNoDuplicates([onp]);
+        assert PathValid(c, [onp]) by {reveal PathValid();}
+        assert PathInSubcircuit([onp], e1.sc) by {reveal PathInSubcircuit();}
         EvaluateONPInnerComposed1(c, e1, e2, path, [onp], knowns);
         assert (EvaluateONPInner(c, [onp], knowns) == EvaluateONPInner(c, [onp], knowns_1)); //  (1)
-        assert (EvaluateONPInner(c, path + [onp], knowns) == EvaluateONPInner(c, [onp], knowns)); // (2)
+        assert (Simpl(EvaluateONPInner(c, path + [onp], knowns)) == Simpl(EvaluateONPInner(c, [onp], knowns))); // (2)
         assert EvaluateINPInner(c, path, knowns) == EvaluateONPInner(c, path + [onp], knowns); // (3)
-        assert knowns_2[np] == e1.f(knowns_1)[onp]; // (4)
-        assert EvaluateONPInner(c, [onp], knowns_1) == EvalOk(e1.f(knowns_1)[onp]); // (5)
+        assert onp in e1.outputs by {
+          reveal ComposedValid();
+          reveal EquivValid();
+          reveal EquivScOutputsInOutputs();
+          assert (np.n !in e1.sc) && np in c.PortSource && c.PortSource[np].n in e1.sc;
+          assert onp in ScOutputBoundary(c, e1.sc);
+        }
+        assert (e1.f.requires(knowns_1)) && (e1.f(knowns_1).Keys == e1.outputs) && (knowns_2[np] == e1.f(knowns_1)[onp]) by { // (4)
+          reveal ComposedValid();
+          reveal EquivValid();
+          reveal MapFunctionValid();
+          assert knowns_1.Keys == e1.inputs;
+          assert e1.f.requires(knowns_1);
+          assert e1.f(knowns_1).Keys == e1.outputs;
+        }
+        assert EvaluateONPInner(c, [onp], knowns_1) == EvalOk(e1.f(knowns_1)[onp]) by { // (5)
+          reveal ComposedValid();
+          reveal EquivTrue();
+        }
 
         assert EvaluateINPInner(c, path, knowns_2) == EvalOk(knowns_2[np]); // by it's own def
         assert EvaluateINPInner(c, path, knowns_2) == EvaluateONPInner(c, [onp], knowns_1); // by (4) and (5)
@@ -259,14 +442,32 @@ module ComposeEval {
         assert EvaluateINPInner(c, path, knowns_2) == EvaluateINPInner(c, path, knowns); // by (3)
       }
     } else {
+      assert np !in e2.inputs;
+      assert knowns_2.Keys == e2.inputs;
+      assert np !in knowns_2;
+      InE2ButNotE2InputsNotInKnowns(c, e1, e2, knowns, np);
+      assert np !in knowns;
       if np in c.PortSource {
         var onp := c.PortSource[np];
-        assert onp.n in e2.sc;
+        assert ONPValid(c, onp) by {
+          reveal CircuitValid();
+        }
+        assert onp.n in e2.sc by {
+          assert np !in e2.inputs;
+          reveal ComposedValid();
+          reveal EquivValid();
+          assert np !in ScInputBoundary(c, e2.sc);
+          assert np !in NPBetweenSubcircuitsComplement(c, e2.sc, e2.sc);
+          assert !(np.n in e2.sc && np in c.PortSource && c.PortSource[np].n !in e2.sc);
+        }
         if onp in path {
           assert EvaluateINPInner(c, path, knowns) == EvaluateINPInner(c, path, knowns_2);
         } else {
           NodesNotInPathDecreases(c, path, onp);
           StillHasNoDuplicates(path, onp);
+          assert PathInSubcircuit(path + [onp], e2.sc) by {
+            reveal PathInSubcircuit();
+          }
           EvaluateONPInnerComposed2(c, e1, e2, path + [onp], knowns);
           assert EvaluateINPInner(c, path, knowns) == EvaluateINPInner(c, path, knowns_2);
         }
@@ -276,28 +477,40 @@ module ComposeEval {
     }
   }
 
-  lemma {:vcs_split_on_every_assert} EvaluateONPInnerComposed1(c: Circuit, e1: Equiv, e2: Equiv, prepath: seq<NP>, path: seq<NP>, knowns: map<NP, bool>)
+  lemma EvaluateONPInnerComposed1(c: Circuit, e1: Equiv, e2: Equiv, prepath: seq<NP>, path: seq<NP>, knowns: map<NP, bool>)
     requires CircuitValid(c)
     requires ComposedValid(c, e1, e2)
-    requires knowns.Keys == ComposeEquivInputs(c, e1, e2)
+    requires GoodKnownKeys(c, e1, e2, knowns)
     requires EvaluateONPInnerRequirements(c, prepath + path, knowns)
     requires EvaluateONPInnerRequirements(c, path, knowns)
-    requires forall np :: np in path ==> np.n in e1.sc
-    requires forall np :: np in prepath ==> np.n in e2.sc
+    requires PathInSubcircuit(path, e1.sc)
+    requires PathInSubcircuit(prepath, e2.sc)
     ensures
+      (forall np :: np in e1.inputs ==> np in knowns) &&
       var knowns_1 := ExtractMap(knowns, e1.inputs);
       (EvaluateONPInner(c, path, knowns) == EvaluateONPInner(c, path, knowns_1)) &&
       (Simpl(EvaluateONPInner(c, prepath + path, knowns)) == Simpl(EvaluateONPInner(c, path, knowns)))
-    decreases |NodesNotInPath(c, prepath + path)|, 4
+    decreases |NodesNotInPath(c, prepath + path)|, 6
   {
-    reveal ComposedValid();
-    reveal EquivValid();
+    assert forall np :: np in e1.inputs ==> np in knowns by {reveal GoodKnownKeys();}
     var knowns_1 := ExtractMap(knowns, e1.inputs);
     var np := Seq.Last(path);
+    assert (np.n in e1.sc) && (np.n !in e2.sc) by {
+      reveal PathInSubcircuit();
+      reveal ComposedValid();
+      InThisNotInThat(np.n, e1.sc, e2.sc);
+    }
     Seq.LemmaAppendLast(prepath, path);
     assert np == Seq.Last(prepath + path);
     if np in knowns {
-      assert np in knowns_1;
+      assert np in knowns_1 by {
+        reveal GoodKnownKeys();
+        reveal ComposedValid();
+        reveal EquivValid();
+        reveal NPsValidAndInSc();
+        assert forall x :: x in e2.inputs ==> x.n in e2.sc;
+        assert np !in e2.inputs;
+      }
       assert EvaluateONPInner(c, path, knowns) == EvaluateONPInner(c, path, knowns_1);
       assert Simpl(EvaluateONPInner(c, prepath + path, knowns)) == Simpl(EvaluateONPInner(c, path, knowns));
     } else {
@@ -322,51 +535,86 @@ module ComposeEval {
     assert Simpl(EvaluateONPInner(c, prepath + path, knowns)) == Simpl(EvaluateONPInner(c, path, knowns));
   }
 
-  lemma {:vcs_split_on_every_assert} EvaluateONPInnerComposed2(c: Circuit, e1: Equiv, e2: Equiv, path: seq<NP>, knowns: map<NP, bool>)
+  lemma EvaluateONPInnerComposed2(c: Circuit, e1: Equiv, e2: Equiv, path: seq<NP>, knowns: map<NP, bool>)
     requires CircuitValid(c)
     requires ComposedValid(c, e1, e2)
-    requires knowns.Keys == ComposeEquivInputs(c, e1, e2)
+    requires GoodKnownKeys(c, e1, e2, knowns)
     requires EvaluateONPInnerRequirements(c, path, knowns)
-    requires forall np :: np in path ==> np.n in e2.sc
+    requires PathInSubcircuit(path, e2.sc)
     ensures
       var knowns_2 := CalculateE2Inputs(c, e1, e2, knowns);
-      var np := path[|path|-1];
+      var np := Seq.Last(path);
       (EvaluateONPInner(c, path, knowns) == EvaluateONPInner(c, path, knowns_2))
-    decreases |NodesNotInPath(c, path)|, 4
+    decreases |NodesNotInPath(c, path)|, 6
   {
-    reveal ComposedValid();
-    reveal EquivValid();
     var knowns_2 := CalculateE2Inputs(c, e1, e2, knowns);
     var np := Seq.Last(path);
+    assert (np.n in e2.sc) && (np.n !in e1.sc) by {
+      reveal PathInSubcircuit();
+      reveal ComposedValid();
+      InThisNotInThat(np.n, e2.sc, e1.sc);
+    }
     if np in knowns {
-      assert np in knowns_2;
+      assert np in knowns_2 by {
+        reveal GoodKnownKeys();
+        reveal ComposedValid();
+        reveal EquivValid();
+        reveal NPsValidAndInSc();
+        assert np !in e1.inputs;
+      }
       assert EvaluateONPInner(c, path, knowns) == EvaluateONPInner(c, path, knowns_2);
     } else {
+      assert np !in e2.inputs by {
+        reveal GoodKnownKeys();
+        reveal ComposedValid();
+        reveal EquivValid();
+        reveal NPsValidAndInSc();
+        reveal CircuitValid();
+        assert knowns.Keys == (e1.inputs + e2.inputs) - NPBetweenSubcircuits(c, e2.sc, e1.sc);
+        assert np !in NPBetweenSubcircuits(c, e2.sc, e1.sc);
+      }
       var nk := c.NodeKind[np.n];
+      assert !nk.CInput? && !nk.CSeq? by {
+        reveal GoodKnownKeys();
+        reveal EquivValid();
+        if (nk.CInput? || nk.CSeq?) {
+          reveal ComposedValid();
+          assert np in InternalInputs(c, e2.sc);
+          assert np in e2.inputs;
+        }
+      }
       match nk
         case CXor() => {
           EvaluateONPBinaryComposed2(c, e1, e2, path, knowns);
+      assert EvaluateONPInner(c, path, knowns) == EvaluateONPInner(c, path, knowns_2);
         }
         case CAnd() => {
           EvaluateONPBinaryComposed2(c, e1, e2, path, knowns);
+      assert EvaluateONPInner(c, path, knowns) == EvaluateONPInner(c, path, knowns_2);
         }
         case CInv() => {
           EvaluateONPUnaryComposed2(c, e1, e2, path, knowns);
+      assert EvaluateONPInner(c, path, knowns) == EvaluateONPInner(c, path, knowns_2);
         }
-        case CConst(b) => {}
+        case CConst(b) => {
+      assert EvaluateONPInner(c, path, knowns) == EvaluateONPInner(c, path, knowns_2);
+
+        }
         case CInput() => {}
         case CSeq() => {}
+      assert EvaluateONPInner(c, path, knowns) == EvaluateONPInner(c, path, knowns_2);
     }
   }
 
-  lemma {:vcs_split_on_every_assert} EvaluateComposedInner(c: Circuit, e1: Equiv, e2: Equiv, np: NP, knowns: map<NP, bool>)
+  lemma EvaluateComposedInner(c: Circuit, e1: Equiv, e2: Equiv, np: NP, knowns: map<NP, bool>)
     requires CircuitValid(c)
     requires ComposedValid(c, e1, e2)
-    requires knowns.Keys == ComposeEquivInputs(c, e1, e2)
+    requires GoodKnownKeys(c, e1, e2, knowns)
     requires ONPValid(c, np) || INPValid(c, np)
     requires np.n in (e1.sc + e2.sc)
     requires np in e1.outputs || np in e2.outputs
     ensures
+      (forall np :: np in e1.inputs ==> np in knowns) &&
       var knowns_1 := ExtractMap(knowns, e1.inputs);
       var knowns_2 := CalculateE2Inputs(c, e1, e2, knowns);
       (np.n in e1.sc ==> Evaluate(c, np, knowns_1) == Evaluate(c, np, knowns)) &&
@@ -374,14 +622,24 @@ module ComposeEval {
   {
     var prepath: seq<NP> := [];
     var path := [np];
-    assert np == path[|path|-1];
-    assert PathValid(c, path);
+    assert np == Seq.Last(path);
+    assert PathValid(c, path) && PathValid(c, prepath + path) by {
+      reveal PathValid();
+    }
 
+    assert forall np :: np in e1.inputs ==> np in knowns by {reveal GoodKnownKeys();}
     var knowns_1 := ExtractMap(knowns, e1.inputs);
     var knowns_2 := CalculateE2Inputs(c, e1, e2, knowns);
 
     LengthOneNoDuplicates(path);
     LengthOneNoDuplicates(prepath + path);
+    if np.n in e1.sc {
+      assert PathInSubcircuit(prepath, e2.sc) by { reveal PathInSubcircuit(); }
+      assert PathInSubcircuit(path, e1.sc) by { reveal PathInSubcircuit(); }
+    } else {
+      assert PathInSubcircuit(path, e2.sc) by { reveal PathInSubcircuit(); }
+    }
+
     if ONPValid(c, np) {
       if np.n in e1.sc {
         EvaluateONPInnerComposed1(c, e1, e2, prepath, path, knowns);
@@ -401,6 +659,7 @@ module ComposeEval {
     }
     reveal ComposedValid();
     if np.n in e1.sc {
+      InThisNotInThat(np.n, e1.sc, e2.sc);
       assert np.n !in e2.sc;
       assert Evaluate(c, np, knowns) == Evaluate(c, np, knowns_1);
     } else {
@@ -409,10 +668,10 @@ module ComposeEval {
     }
   }
 
-  lemma {:vcs_split_on_every_assert} EvaluateComposed(c: Circuit, e1: Equiv, e2: Equiv, np: NP, knowns: map<NP, bool>)
+  lemma EvaluateComposed(c: Circuit, e1: Equiv, e2: Equiv, np: NP, knowns: map<NP, bool>)
     requires CircuitValid(c)
     requires ComposedValid(c, e1, e2)
-    requires knowns.Keys == ComposeEquivInputs(c, e1, e2)
+    requires GoodKnownKeys(c, e1, e2, knowns)
     requires ONPValid(c, np) || INPValid(c, np)
     requires np.n in (e1.sc + e2.sc)
     requires np in e1.outputs || np in e2.outputs
@@ -425,30 +684,55 @@ module ComposeEval {
     EvaluateComposedInner(c, e1, e2, np, knowns);
     var e := ComposeEquiv(c, e1, e2);
     assert EquivValid(c, e);
-    {
-      reveal EquivValid();
-      assert e.f.requires(knowns);
-      assert np in e.f(knowns);
-    }
 
     var knowns_1 := ExtractMap(knowns, e1.inputs);
     var knowns_2 := CalculateE2Inputs(c, e1, e2, knowns);
 
+    assert e1.f.requires(knowns_1) && (e1.f(knowns_1).Keys == e1.outputs) &&
+           e2.f.requires(knowns_2) && (e2.f(knowns_2).Keys == e2.outputs) &&
+           e.f.requires(knowns) && (e.f(knowns).Keys == e.outputs) by {
+      reveal ComposedValid();
+      reveal EquivValid();
+      reveal MapFunctionValid();
+      reveal GoodKnownKeys();
+      assert EquivValid(c, e1);
+      assert EquivValid(c, e2);
+      assert EquivValid(c, e);
+      assert e.f.requires(knowns);
+      assert (e.f(knowns).Keys == e.outputs);
+    }
     if np in e1.outputs {
-      {
+      assert np.n in e1.sc by {
         reveal ComposedValid();
         reveal EquivValid();
-        assert Evaluate(c, np, knowns_1) == EvalOk(e1.f(knowns_1)[np]);
+        reveal NPsValidAndInSc();
+      }
+      assert Evaluate(c, np, knowns_1) == EvalOk(e1.f(knowns_1)[np]) by {
+        reveal ComposedValid();
+        assert EquivTrue(c, e1);
+        reveal EquivTrue();
       }
       assert Evaluate(c, np, knowns) == Evaluate(c, np, knowns_1);
-      assert EvalOk(e1.f(knowns_1)[np]) == EvalOk(e.f(knowns)[np]);
+      assert EvalOk(e1.f(knowns_1)[np]) == EvalOk(e.f(knowns)[np]) by {
+        reveal GoodKnownKeys();
+        reveal ComposedValid(); reveal EquivTrue();
+      }
       assert Evaluate(c, np, knowns) == EvalOk(e.f(knowns)[np]);
     } else {
       assert np in e2.outputs;
-      {
+      assert np.n in e2.sc by {
         reveal ComposedValid();
         reveal EquivValid();
-        assert Evaluate(c, np, knowns_2) == EvalOk(e2.f(knowns_2)[np]);
+        reveal NPsValidAndInSc();
+      }
+      assert Evaluate(c, np, knowns_2) == EvalOk(e2.f(knowns_2)[np]) by {
+        reveal ComposedValid();
+        reveal EquivTrue();
+      }
+      assert EvalOk(e2.f(knowns_2)[np]) == EvalOk(e.f(knowns)[np]) by {
+        reveal GoodKnownKeys();
+        reveal ComposedValid();
+        reveal EquivTrue();
       }
       assert Evaluate(c, np, knowns) == Evaluate(c, np, knowns_2);
       assert EvalOk(e2.f(knowns_2)[np]) == EvalOk(e.f(knowns)[np]);
@@ -457,7 +741,7 @@ module ComposeEval {
     }
   }
 
-  lemma {:vcs_split_on_every_assert} ComposeEquivCorrect(c: Circuit, e1: Equiv, e2: Equiv)
+  lemma ComposeEquivCorrect(c: Circuit, e1: Equiv, e2: Equiv)
     requires ComposedValid(c, e1, e2)
     ensures
       var r := ComposeEquiv(c, e1, e2);
@@ -475,17 +759,24 @@ module ComposeEval {
         e.f.requires(knowns) &&
         (forall np :: np in e.outputs ==>
           np in e.f(knowns) &&
+          NPValid(c, np) &&
           (Evaluate(c, np, knowns) == EvalOk(e.f(knowns)[np])))
     {
       forall np | np in e.outputs
         ensures
           e.f.requires(knowns) &&
           np in e.f(knowns) &&
+          NPValid(c, np) &&
           (Evaluate(c, np, knowns) == EvalOk(e.f(knowns)[np]))
       {
+        reveal ComposedValid();
+        reveal GoodKnownKeys();
+        reveal EquivValid();
+        reveal NPsValidAndInSc();
         EvaluateComposed(c, e1, e2, np, knowns);
       }
     }
+    reveal EquivTrue();
     assert EquivTrue(c, e);
   }
 
