Attempt2/HideOutput.dfy
@@ -3,6 +3,7 @@ module HideOutput {
   import opened Circ
   import opened Equiv
   import opened Utils
+  import opened MapFunction
 
   function EquivHideOutput(c: Circuit, e: Equiv, remove: set<NP>): (r: Equiv)
     requires CircuitValid(c)
@@ -11,7 +12,13 @@ module HideOutput {
     ensures EquivValid(c, r)
     ensures EquivTrue(c, e) ==> EquivTrue(c, r)
   {
+    reveal CircuitValid();
     reveal EquivValid();
+    reveal EquivTrue();
+    reveal ScValid();
+    reveal NPsValidAndInSc();
+    reveal EquivScOutputsInOutputs();
+    reveal MapFunctionValid();
     Equiv(e.sc, e.inputs, e.outputs - remove, (x: map<NP, bool>) requires x.Keys == e.inputs => e.f(x) - remove)
   }
 
